Adapt to visibility in Pulse.

src/lib/kuiper/Kuiper.ArrayCoreAssumptions.fsti
@@ -7,29 +7,3 @@ module SZ = FStar.SizeT
 //we could expose this from core_pcm_ref
 //assuming that every allocation is at least 128-aligned
 val core_base_address (x:A.array 'a) : GTot (n:nat { n > 0 /\ n%128==0 })
-
-let visibility = loc_id -> loc_id
-
-val loc_id_of_array (#a:Type u#a) (x:A.array a) : loc_id
-
-val visibility_of_array (#a:Type u#a) (x:A.array a) : visibility
-
-let array_visible_at (#a:Type) (x:A.array a) (l:loc_id) =
-  visibility_of_array x l ==
-  visibility_of_array x (loc_id_of_array x)
-
-fn alloc_array_with_vis u#a (#elt: Type u#a) {| small_type u#a |} 
-      (x: elt) (n: SZ.t) (l:loc_id)
-      (vis:visibility)
-  requires loc l
-  returns a: array elt
-  ensures loc l
-  ensures pts_to_mask a (Seq.create (SZ.v n) x) (fun _ -> True)
-  ensures pure (
-    A.length a == SZ.v n /\
-    A.is_full_array a /\
-    visibility_of_array a == vis /\
-    loc_id_of_array a == l)
-
-val is_send_across_pts_to_mask (#a: Type u#a) (x:A.array a) (f:perm) (s:Seq.seq a) (mask:nat -> prop)
-: is_send_across (visibility_of_array x) (pts_to_mask x #f s mask)
